coq/minor.v
@@ -329,3 +329,65 @@ Proof.
   apply: leq_trans wT. apply: leq_trans B2. exact: K4_width.
 Qed.
 
+Section AddNode.
+  Variables (G : sgraph) (N : {set G}).
+  
+  Definition add_node_rel (x y : option G) := 
+    match x,y with 
+    | None, Some y => y \in N
+    | Some x, None => x \in N
+    | Some x,Some y => x -- y
+    | None, None => false
+    end.
+
+  Lemma add_node_sym : symmetric add_node_rel.
+  Proof. move => [a|] [b|] //=. by rewrite sgP. Qed.
+
+  Lemma add_node_irrefl : irreflexive add_node_rel.
+  Proof. move => [a|] //=. by rewrite sgP. Qed.
+
+  Definition add_node := SGraph add_node_sym add_node_irrefl.
+End AddNode.
+Arguments add_node : clear implicits.
+
+
+Lemma minor_with (H G': sgraph) (S : {set H}) (i : H) (N : {set G'})
+  (phi : (sgraph.induced S) -> option G') : 
+  i \notin S -> 
+  (forall y, y \in N -> exists2 x , x \in phi @^-1 (Some y) & val x -- i) ->
+  @minor_map (sgraph.induced S) G' phi -> 
+  minor H (add_node G' N).
+Proof.
+  move => Hi Hphi mm_phi.
+  pose psi (u:H) : option (add_node G' N) := 
+    match @idP (u \in S) with 
+    | ReflectT p => obind (fun x => Some (Some x)) (phi (Sub u p))
+    | ReflectF _ => if u == i then Some None else None
+    end.
+  (* NOTE: use (* case: {-}_ / idP *) to analyze psi *)
+  have psi_G' (a : G') : psi @^-1 (Some (Some a)) = val @: (phi @^-1 (Some a)).
+  { apply/setP => x. rewrite !inE. apply/eqP/imsetP.
+    + rewrite /psi. case: {-}_ / idP => p; last by case: ifP. 
+      case E : (phi _) => [b|//] /= [<-]. exists (Sub x p) => //. by rewrite !inE E.
+    + move => [[/= b Hb] Pb] ->. rewrite /psi. case: {-}_ / idP => //= Hb'. 
+      rewrite !inE (bool_irrelevance Hb Hb') in Pb. by rewrite (eqP Pb). }
+  have psi_None : psi @^-1 (Some None) = [set i].
+  { apply/setP => z. rewrite !inE /psi. 
+    case: {-}_ / idP => [p|_]; last by case: ifP.
+    have Hz : z != i. { apply: contraNN Hi. by move/eqP <-. }
+    case: (phi _) => [b|]; by rewrite (negbTE Hz). }
+  case: mm_phi => M1 M2 M3. exists psi;split.
+  - case. 
+    + move => a. case: (M1 a) => x E. exists (val x). apply/eqP. 
+      rewrite mem_preim psi_G' mem_imset //. by rewrite !inE E. 
+    + exists i. rewrite /psi. move: Hi. 
+      case: {-}_ / idP => [? ?|_ _]; by [contrab|rewrite eqxx].
+  - case. 
+    + move => y. move: (M2 y). rewrite psi_G'. exact: connected_in_subgraph.
+    + rewrite psi_None. exact: connected1.
+  - move => [a|] [b|]; last by rewrite sg_irrefl.
+    + move => /= /M3 [x0] [y0] [? ? ?]. 
+      exists (val x0). exists (val y0). by rewrite !psi_G' !mem_imset.
+    + move => /= /Hphi [x0] ? ?. exists (val x0); exists i. by rewrite psi_None set11 !psi_G' !mem_imset.
+    + move => /= /Hphi [x0] ? ?.  exists i;exists (val x0). by rewrite sg_sym psi_None set11 !psi_G' !mem_imset.
+Qed.
